Argyle/Logic/InhibitionNet.lean
@@ -1,0 +1,59 @@
+import Mathlib.Data.Fintype.Basic
+import Mathlib.Data.Rel
+import Argyle.Helpers
+
+-- Inhibition Nets, an implementation of Hannes' construction
+-- following his paper:
+--    "Nonmonotonic reasoning by inhibition nets" (2001)
+--
+-- An Inhibition Net is a special net that has no weights,
+-- but inhibitory synapses control the flow of activation).
+-- It turns out that binary ANNs are equivalent to
+-- Inhibition Nets (the inhibitory synapses simulate
+-- negative weights).
+--
+-- An inhibitory edge connects a node to an excitatory edge, e.g.:
+--
+--         a --------> b
+--               |
+--               |
+--         c ----⧸
+--
+-- Additionally, there are no weights or activation functions.
+-- Excitatory edges always go through, unless some inhibitory
+-- edge is currently preventing it from going through.
+-- There are three types of edges:
+--   - Edge: Do nothing, act as a "skeleton" for excitatory edges.
+--   - Excit: Excitatory edges that always go through, unless inhibited
+--   - Inhib: Inhibitory edges that prevent excitatory edges from going through
+
+-- NOTE: As with InterpretedNets, we add a proposition mapping
+-- as well.  We also have a 'bias' node, which occurs in *every*
+-- activation.
+structure InhibitionNet (Node : Type) where
+  Edge : Rel Node Node -- NOTE: Skeleton edges do nothing; they just specify
+                           -- where the excitatory edges can be
+  Excit : Rel Node Node
+  Inhib : Rel Node (Node × Node) -- need to be connected to excitatory_edges!!!
+  proposition_map : String → Set Node
+
+  -- There are finitely many nodes, and there is some node 'bias' ∈ Node.
+  -- (bias is a node which shows up in the propagation of every signal.)
+  nodes : Fintype Node
+  bias : Node
+
+  -- The graph is nonempty, acyclic and fully connected.
+  acyclic : Acyclic Edge
+  connected : Connected Edge
+
+  -- The relationships between each of the edge types
+  excit_edge : ∀ (m n : Node), Excit m n → Edge m n
+  inhib_excit : ∀ (b m n : Node), Inhib b ⟨m, n⟩ → Excit m n
+
+-- Propagation in an Inhibition Net
+-- Essentially, n is active iff some node m excites n
+-- and there is no inhibitory node b that stops this activation.
+-- Note that the 'bias' node always activates.
+def InhibitionNet.propagate (net : InhibitionNet Node) (S : Set Node) : Set Node :=
+  fun n => n ∈ S ∨ (n = net.bias) ∨
+    ∃ m, net.Excit m n ∧ ¬∃ b, net.Inhib b ⟨m, n⟩
